# Assignment One

| Name:           | 汪明杰  |
| --------------- | ------- |
| Student Number: | 1851055 |



## 1

当n变为原来的4倍时:

**a. ** $$ log_2n$$ 将变为原来的 $$ \frac{log_2 {4n}}{log_2 n} =\frac{2+log_2n}{log_2n} = 1+ \frac{2}{log_2n}$$ 倍。

**b. ** $$\sqrt n$$ 将变为原来的$$ \frac{\sqrt{4n}}{\sqrt n} = \sqrt 4=2 $$ 倍。

**c.**   $$n$$将变为原来的$$ \frac{4n}{n}=4$$ 倍。

**d.**  $$n^2$$ 将变为原来的$$\frac {(4n)^2}{n^2}=4^2=16$$ 倍。

**e.**  $$ n^3$$将变为原来的$$ \frac {(4n)^3}{n^3}=4^3=64 $$ 倍。

**f.**  $$ 2^n $$ 将变为原来的$$ \frac{2^{4n}}{2^n} = 2^{4n-n} =2^{3n}$$ 倍。



## 2

**a.** Prove:
$$
\because t(n)\in O(g(n)),
\\\therefore\exist n_0使得n>n_0,t(n)\leq cg(n)(c>0),
\\即\exist n_0使得n>n_0,g(n)\geq \frac{1}{c}t(n).
\\不妨令c'=\frac{1}{c},
\\也即\exist n_0使得n>n_0,g(n)\geq c't(n).
\\\therefore g(n) \in \Omega(t(n)).
$$
**b.**Prove:
$$
\forall  t(n) \in \Theta(g(n)),
\\即 \forall n>n_0, c_2g(n)\leq t(n) \leq c_1 g(n).
\\ 不妨取c_3= \frac{1}{\alpha}c_2, c_4=\frac{1}{\alpha}c_1,
\\则有\forall n>n_0, \alpha c_3 g(n)\leq t(n) \leq \alpha c_4 g(n).
\\ \therefore t(n) \in \Theta(\alpha g(n)).
\\\therefore \Theta(g(n)) \subseteq \Theta(\alpha g(n)).
\\同理可证， \Theta(\alpha g(n)) \subseteq \Theta(g(n)).
\\ \therefore \Theta(\alpha g(n)) = \Theta(g(n)),\alpha >0.
$$
**c.**Prove:
$$
\forall t(n) \in O(g(n)) \cap \Omega(g(n)),
\\有 \forall n>n_1,t(n) \leq c_1g(n) ;\forall n>n_2,t(n)\geq c_2g(n).
\\不妨取n_0=max\{ n_1,n_2\},
\\则\forall n>n_0, t(n) \leq c_1g(n) 且t(n)\geq c_2g(n),
\\ \therefore t(n) \in \Theta (g(n)),
\\ \therefore O(g(n)) \cap \Omega(g(n)) \subseteq \Theta(g(n)).
\\同理可证, \Theta(g(n)) \subseteq O(g(n)) \cap \Omega(g(n)).
\\ \therefore \Theta(g(n)) = O(g(n)) \cap \Omega(g(n)).
$$

**d.** Disprove:
$$
取t(n)=\begin{cases}2^n,当n为奇数时\\2^{-n},当n为偶数时\end{cases},g(n)=n.
\\显然满足t(n)>0 \ \ and\ \ g(n)>0.


\\当n为奇数时,\lim_{n \to +\infty} \frac{ct(n)}{g(n)}=\lim_{n \to +\infty}\frac{c\cdot2^n}{n}>1,即\ ct(n)>g(n);
\\而当n为偶数时,\lim_{n \to +\infty} \frac{ct(n)}{g(n)}=\lim_{n \to +\infty}\frac{c\cdot2^{-n}}{n}<1,即\ ct(n)<g(n).
\\ \therefore \not\exist n_0使得n>n_0时,
\\满足t(n) \leq c_1g(n) \ \  or \ \ t(n) \geq c_2g(n). \\ \therefore t(n) \not\in O(g(n)) \ \ and\ \  t(n) \not \in \Omega(g(n)). \\ \therefore原命题为假命题.
$$

## 3

**a.**Solve:
$$
\because x(n) =3x(n-1),
\\ \therefore x(n)=3x(n-1)=3^2x(n-1)=3^3x(n-2)
\\=\cdots
\\=3^{n-1} x(1).
\\ \because x(1)=4,
\\ \therefore x(n)=4*3^{n-1}.
$$
**b.**Solve:
$$
\because x(n)=x(n-1)+n,
\\ \therefore x(n)=n+x(n-1)
\\=n+(n-1)+x(n-2)
\\=\cdots
\\=n+(n-1)+\cdots +1+x(0)
\\=\sum^{n}_{i=1}i+x(0).
\\ \because x(0)=0\ and\ \sum^{n}_{i=1}i= \frac{n(n+1)}{2}，
\\\therefore x(n)=\frac{n(n+1)}{2}.
$$
**c.**Solve:
$$
\because n=2^k,x(n)=x(\frac{n}{2})+n,
\\ \therefore x(2^k)=x(\frac{2^k}{2})+2^k=x(2^{k-1})+2^k
\\=2^k+2^{k-1}+x(2^{k-2})
\\=\cdots
\\=2^k+2^{k-1}+\cdots+2^2+2^1+x(2^0).
\\\because x(2^0)=x(1)=1,\sum_{i=1}^{k}2^i=2(2^k-1),
\\ \therefore x(2^k)=2*2^k-1.
\\ \because n=2^k,
\\ \therefore x(n)=2n-1.
$$
